\documentclass[a4paper]{article}
\author{Piotr Marzec 3 GRP}
\title{Ä†wiczenia nr.4 Latex}
\usepackage[left=3.5cm, right=2.5cm, top=2.5cm, bottom=2.5cm]{geometry}
\usepackage[MeX]{polski}
\usepackage[utf8]{inputenc}
\usepackage{graphicx}
\usepackage{enumerate}
\usepackage{amsmath} %pakiet matematyczny
\usepackage{amssymb} %pakiet dodatkowych symboli
\usepackage{float}
\begin{document}
$$
\begin{cases}
	\mid z \mid = \mid z-4i\mid \\
	\frac{\pi}{4}\geq Arg z < \frac{\pi}{2} \\
\end{cases}
$$
$$
	\begin{cases}
	\mid z+4 \mid = \mid z+2-2i \mid \\
	\mid z \mid\ \geq 2
	\end{cases}
$$
$$
\begin{cases}
\mid z - 1 - i \mid < \sqrt{2} \\
Arg(z-1-i)<\frac{\pi}{2} \\
\end{cases}
$$
$$
\begin{cases}
x+5y=2\\
-3x+6y=15\\
\end{cases}
$$
$$
\left\{
\begin{array}{rrrrrrr}
x&-&y&-&z&=&1\\
3x&+&4y&-&2z&=&-1\\
3x&-&2y&-&2z&=&1\\
\end{array}
\right.
$$
$$
\left\{
\begin{array}{rrrrrrrrr}
&&y&-&3z&+&4v&=&0\\
x&&&-&2z&&&=&0\\
3x&+&2y&&&-&5v&=&2\\
4x&&&-&5z&&&=&0
\end{array}
\right.
$$
$$
\begin{bmatrix}
1&0&0\\
0&3&0\\
0&0&1\\
\end{bmatrix} * \begin{bmatrix}
				1&2&3\\
				3&1&2\\
				5&1&3\\
				\end{bmatrix}
$$
$$
\begin{bmatrix}
0&1&0\\
1&0&0\\
0&0&1\\
\end{bmatrix} * \begin{bmatrix}
				11&-2\\
				6&-14\\
				-21&30\\
				\end{bmatrix}
$$
$$
\begin{bmatrix}
1&0&0\\
0&1&0\\
1&0&1\\
\end{bmatrix} * \begin{bmatrix}
					1&1&3\\
					2&1&4\\
					1&3&0
				\end{bmatrix}
$$
$$
\begin{vmatrix}
-3&2\\
8&-5\\
\end{vmatrix}
$$
$$
\begin{vmatrix}
\sin\alpha & \cos\alpha\\
\sin\beta & \cos\beta\\
\end{vmatrix}
$$
$$
\begin{vmatrix}
1&i&1+i\\
-i&1&0\\
1-i&0&1\\
\end{vmatrix}
$$
$$
\left[
\begin{array}{c|cc|ccc}
1&0&0&1&1&1\\
\hline
0&2&2&1&2&3\\
0&2&2&4&5&6\\
\hline
0&0&0&3&3&1\\
0&0&0&3&1&3\\
0&0&0&1&3&3\\
\end{array}
\right]
$$
$$\int^\infty_1 \frac{dx}{(x+2)^2}$$
$$\int^0_{-\infty}\frac{dx}{x^2+4}$$
$$\int^\infty_{-\infty}x^2exp^{-x^3}dx$$
$$\int^\infty_1 \frac{dx}{\sqrt[3]{3x+5}}$$
$$log_{\sqrt{5}}5\sqrt[3]{5}$$
$$log_{\sqrt[3]{3}}27$$
$$log_2 8\sqrt{2}$$
$$\lim_{n\to\infty}(\sqrt{n+6\sqrt{n}+1}-\sqrt{n})$$
$$\lim_{n\to\infty} \frac{1+\frac{1}{2}+\frac{1}{2^2}+\ldots+\frac{1}{2^n}}{1+\frac{1}{3}+\frac{1}{3^2}+\ldots+\frac{1}{3^n}}$$
$$\sum_{n=1}^\infty (-1)^{n+1}(2n-1)$$
$$\sum_{n=1}^\infty \sin\frac{2\pi}{3^n}\cos\frac{4\pi}{3^n}$$
$$
\begin{bmatrix}
1&2&3\\
0&-6&7
\end{bmatrix}^T=\begin{bmatrix}
					1&0\\
					2&-6\\
					3&7
				\end{bmatrix}
$$
$$
U_{AB}=\frac{W_{A \to B}}{q} =\int_A^B\vec{E} *\vec{dl}
$$
\end{document}